Added example of program verification

theories/Semantics/IMP/Axiomatic.v
@@ -1,7 +1,8 @@
 From stdpp Require Import prelude.
+From Coq Require Import Classical.
 From sets Require Import Functions Ensemble.
 
-From Semantics Require Import Syntax State Eval.
+From Semantics Require Import Syntax State Denotational.
 
 Inductive EAExp : Type :=
     | LVar : nat -> EAExp
@@ -18,6 +19,26 @@ Fixpoint aexp_to_eaexp (a : AExp) : EAExp :=
   | Plus a1 a2 => EPlus (aexp_to_eaexp a1)  (aexp_to_eaexp a2)
   | Minus a1 a2 => EMinus (aexp_to_eaexp a1)  (aexp_to_eaexp a2)
   | Mul a1 a2 => EMul (aexp_to_eaexp a1)  (aexp_to_eaexp a2)
+  end.
+
+Fixpoint aloc_vars (a : EAExp) : Ensemble nat :=
+  match a with
+  | EAVal z => ∅
+  | EVar x => {[x]}
+  | LVar x => ∅
+  | EPlus a1 a2 => aloc_vars a1 ∪ aloc_vars a2
+  | EMinus a1 a2 => aloc_vars a1 ∪ aloc_vars a2
+  | EMul a1 a2 => aloc_vars a1 ∪ aloc_vars a2
+  end.
+
+Fixpoint alog_vars (a : EAExp) : Ensemble nat :=
+  match a with
+  | EAVal z => ∅
+  | EVar x => ∅
+  | LVar x => {[x]}
+  | EPlus a1 a2 => alog_vars a1 ∪ alog_vars a2
+  | EMinus a1 a2 => alog_vars a1 ∪ alog_vars a2
+  | EMul a1 a2 => alog_vars a1 ∪ alog_vars a2
   end.
 
 Coercion aexp_to_eaexp : AExp >-> EAExp.
@@ -45,6 +66,28 @@ Fixpoint bexp_to_ebexp (b : BExp) : EBExp :=
   | Or b1 b2 => EOr (bexp_to_ebexp b1) (bexp_to_ebexp b2)
   end.
 
+Fixpoint bloc_vars (b : EBExp) : Ensemble nat :=
+  match b with
+  | EBVal t => ∅
+  | EAEq a1 a2 => aloc_vars a1 ∪ aloc_vars a2
+  | EALe a1 a2 => aloc_vars a1 ∪ aloc_vars a2
+  | ENot b => bloc_vars b
+  | EAnd b1 b2 => bloc_vars b1 ∪ bloc_vars b2
+  | EOr b1 b2 => bloc_vars b1 ∪ bloc_vars b2
+  | Forall x b => bloc_vars b
+  end.
+
+Fixpoint blog_vars (b : EBExp) : Ensemble nat :=
+  match b with
+  | EBVal t => ∅
+  | EAEq a1 a2 => alog_vars a1 ∪ alog_vars a2
+  | EALe a1 a2 => alog_vars a1 ∪ alog_vars a2
+  | ENot b => blog_vars b
+  | EAnd b1 b2 => blog_vars b1 ∪ blog_vars b2
+  | EOr b1 b2 => blog_vars b1 ∪ blog_vars b2
+  | Forall x b => blog_vars b ∖ {[x]}
+  end.
+
 Coercion bexp_to_ebexp : BExp >-> EBExp.
 
 Definition substitution : Type := nat -> option AExp.
@@ -60,7 +103,7 @@ Definition asubst (a : EAExp) (logv : substitution) (locv : substitution) : EAEx
   | EMul a1 a2 => EMul (go a1)  (go a2)
   end) a.
 
-Fixpoint bsubst  (b : EBExp) (logv : substitution) (locv : substitution) : EBExp :=
+Fixpoint bsubst  (b : EBExp) (logv locv : substitution) : EBExp :=
   match b with
   | EBVal t => EBVal t
   | EAEq a1 a2 => EAEq (asubst a1 logv locv) (asubst a2 logv locv)
@@ -76,6 +119,93 @@ Definition subst0 : substitution := const None.
 Definition update (subst : substitution) (sub : list (nat * AExp)) : substitution :=
   foldr (fun p s => fn_update s p.1 (Some p.2)) subst sub.
 
+Definition mk_subst := update subst0.
+
+Definition subst_vars (s : substitution) : Ensemble nat :=
+    fun (x : nat) => is_Some (s x).
+
+Lemma subst_vars0 : subst_vars subst0 ≡ ∅.
+Proof. by apply equiv_empty; intros x [a Hx]. Qed.
+
+Lemma subst_vars_fn_update_Some : forall (s : substitution) (x : nat) (a : AExp),
+    subst_vars (fn_update s x (Some a)) ≡ subst_vars s ∪ {[x]}.
+Proof.
+    intros; intro y; rewrite elem_of_union, elem_of_singleton.
+    split.
+    - intros [b Hy].
+      unfold fn_update in Hy.
+      by case_decide; [right | left; eexists].
+    - intros [[b Hy]| ->].
+      + unfold fn_update, subst_vars, elem_of, pow_set_elem_of; cbn.
+        by case_decide; eexists.
+      + by exists a; rewrite fn_update_eq.
+Qed.
+
+Lemma subst_vars_update : forall (s : substitution) (sub : list (nat * AExp)),
+    subst_vars (update s sub) ≡ subst_vars s ∪ list_to_set (map fst sub).
+Proof.
+    intros *; revert s; induction sub; [by set_solver |].
+    intro s; cbn.
+    rewrite subst_vars_fn_update_Some, IHsub.
+    by set_solver.
+Qed.
+
+Lemma subst_vars_mk_subst : forall (sub : list (nat * AExp)),
+    subst_vars (mk_subst sub) ≡ list_to_set (map fst sub).
+Proof.
+    intros; unfold mk_subst.
+    rewrite subst_vars_update, subst_vars0.
+    by set_solver.
+Qed.
+
+Lemma asubst_id : forall (a : EAExp) (slog sloc : substitution),
+    aloc_vars a ∩ subst_vars sloc ≡ ∅ ->
+    alog_vars a ∩ subst_vars slog ≡ ∅ ->
+    asubst a slog sloc = a.
+Proof.
+    intros *; induction a; intros Hloc Hlog.
+    - cbn; cut (slog n = None); [by intros -> |].
+      cbn in Hlog.
+      assert (Hn : n ∉ subst_vars slog) by set_solver.
+      destruct (slog n) eqn:Hslog; [| done].
+      by contradict Hn; eexists.
+    - done.
+    - cbn; cut (sloc n = None); [by intros -> |].
+      cbn in Hloc.
+      assert (Hn : n ∉ subst_vars sloc) by set_solver.
+      destruct (sloc n) eqn:Hslog; [| done].
+      by contradict Hn; eexists.
+    - cbn; setoid_rewrite IHa1; [| by set_solver..].
+      by setoid_rewrite IHa2; [| set_solver..].
+    - cbn; setoid_rewrite IHa1; [| by set_solver..].
+      by setoid_rewrite IHa2; [| set_solver..].
+    - cbn; setoid_rewrite IHa1; [| by set_solver..].
+      by setoid_rewrite IHa2; [| set_solver..].
+Qed.
+
+Lemma bsubst_id : forall (b : EBExp) (slog sloc : substitution),
+    bloc_vars b ∩ subst_vars sloc ≡ ∅ ->
+    blog_vars b ∩ subst_vars slog ≡ ∅ ->
+    bsubst b slog sloc = b.
+Proof.
+    induction b; intros slog sloc Hloc Hlog.
+    - done.
+    - by cbn; rewrite !asubst_id by set_solver.
+    - by cbn; rewrite !asubst_id by set_solver.
+    - by cbn; setoid_rewrite IHb; [| set_solver..].
+    - cbn; setoid_rewrite IHb1; [| by set_solver..].
+      by setoid_rewrite IHb2; [| set_solver..].
+    - cbn; setoid_rewrite IHb1; [| by set_solver..].
+      by setoid_rewrite IHb2; [| set_solver..].
+    - cbn. rewrite IHb; [done | by set_solver |].
+      cbn in Hlog; apply equiv_empty.
+      intro x; rewrite elem_of_intersection; intros [Hx [a Ha]].
+      unfold fn_update in Ha; case_decide; [done |].
+      apply Hlog.
+      rewrite elem_of_intersection, elem_of_difference, elem_of_singleton.
+      by split_and!; [..| eexists].
+Qed.
+
 Definition eaeval (sigma : State) (I : nat -> Z): EAExp -> Z :=
     fix eval (a : EAExp) :=
     match a with
@@ -88,7 +218,7 @@ Definition eaeval (sigma : State) (I : nat -> Z): EAExp -> Z :=
     end.
 
 Lemma eaeval_aexp: forall (a : AExp) (sigma : State) (I : nat -> Z),
-    eaeval sigma I a = aeval sigma a.
+    eaeval sigma I a = denota a sigma.
 Proof.
     intros.
     induction a.
@@ -183,6 +313,10 @@ Lemma satsi_and_elim_r : forall (sigma I : State) (b1 b2 : EBExp),
     satsi sigma I (EAnd b1 b2) -> satsi sigma I b2. 
 Proof. by set_solver. Qed.
 
+Lemma satsi_and : forall (sigma I : State) (b1 b2 : EBExp),
+    satsi sigma I (EAnd b1 b2) <-> satsi sigma I b1 /\ satsi sigma I b2.
+Proof. by set_solver. Qed.
+
 Lemma satsi_or : forall (sigma I : State) (b1 b2 : EBExp),
     satsi sigma I (EOr b1 b2) <-> satsi sigma I b1 \/ satsi sigma I b2.
 Proof. by intros; unfold satsi; cbn; rewrite !top_char, elem_of_union. Qed.
@@ -194,3 +328,242 @@ Proof.
     setoid_rewrite top_char.
     by rewrite elem_of_indexed_intersection.
 Qed.
+
+Lemma satsi_mp :  forall (sigma I : State) (b1 b2 : EBExp),
+    satsi sigma I (eimpl b1 b2) -> satsi sigma I b1 -> satsi sigma I b2.
+Proof.
+    intros *; unfold eimpl.
+    rewrite satsi_or, satsi_not.
+    by intros [].
+Qed.
+
+Lemma classical_satsi_impl :  forall (sigma I : State) (b1 b2 : EBExp),
+    satsi sigma I (eimpl b1 b2) <-> (satsi sigma I b1 -> satsi sigma I b2).
+Proof.
+    split; [by apply satsi_mp |].
+    intros *; unfold eimpl.
+    rewrite satsi_or, satsi_not.
+    intros Himpl.
+    destruct (classic (satsi sigma I b1)).
+    - by right; apply Himpl.
+    - by left.
+Qed.
+
+Lemma satsi_eval : forall (sigma I : State) (b : BExp),
+    satsi sigma I b <-> denotb b sigma = true.
+Proof.
+    intros; induction b.
+    - destruct b; [done |]; cbn.
+      split; [| done].
+      by intro Ha; exfalso; apply top_not_bottom.
+    - setoid_rewrite satsi_eq.
+      rewrite !eaeval_aexp; cbn; unfold denota.
+      by rewrite bool_decide_eq_true.
+    - setoid_rewrite satsi_le.
+      rewrite !eaeval_aexp; cbn; unfold denota.
+      by rewrite bool_decide_eq_true.
+    - setoid_rewrite satsi_not.
+      setoid_rewrite IHb; cbn.
+      rewrite negb_true_iff.
+      by unfold denotb; destruct Eval.beval.
+    - setoid_rewrite satsi_and.
+      setoid_rewrite IHb1; setoid_rewrite IHb2; cbn.
+      by rewrite andb_true_iff.
+    - setoid_rewrite satsi_or.
+      setoid_rewrite IHb1; setoid_rewrite IHb2; cbn.
+      by rewrite orb_true_iff.
+Qed.
+
+Definition sat (b : EBExp) : Prop :=
+    forall (sigma I : State), satsi sigma I b.
+
+Definition sem (I : State) (A : EBExp) : Ensemble State :=
+    fun (sigma : State) => satsi sigma I A.
+
+Record HoareTriple : Type := ht
+{
+    pre_condition : EBExp;
+    command : Cmd;
+    post_condition : EBExp;
+}.
+
+Definition ht_satsi (sigma I : State) (t : HoareTriple) : Prop :=
+    satsi sigma I (pre_condition t) ->
+    forall (sigma' : State), (sigma, sigma') ∈ denotc (command t) ->
+    satsi sigma' I (post_condition t).
+
+Definition ht_sati (I : State) (t : HoareTriple) : Prop :=
+    forall (sigma : State), ht_satsi sigma I t.
+
+Lemma ht_sati_alt: forall (I : State) (t : HoareTriple),
+    ht_sati I t
+      <->
+    forall (sigma sigma' : State), (sigma, sigma') ∈ denotc (command t) ->
+    satsi sigma I (pre_condition t) ->
+    satsi sigma' I (post_condition t).
+Proof.
+    split; [by intros Ht **; eapply Ht |].
+    by intros Hall ? ? **; eapply Hall.
+Qed.
+
+Definition ht_sat (t : HoareTriple) : Prop :=
+    forall (I : State), ht_sati I t.
+
+Inductive ht_ded : EBExp -> Cmd -> EBExp -> Prop :=
+| ht_skip : forall (B : EBExp), ht_ded B Skip B
+| ht_asgn : forall (B : EBExp) (x : nat) (a : AExp),
+    ht_ded (bsubst B subst0 (mk_subst [(x, a)])) (Asgn x a) B
+| ht_seq : forall (A B C : EBExp) (c0 c1 : Cmd),
+    ht_ded A c0 B -> ht_ded B c1 C -> ht_ded A (Seq c0 c1) C
+| ht_if : forall (A B : EBExp) (b : BExp) (c0 c1 : Cmd),
+    ht_ded (EAnd A b) c0 B -> ht_ded (EAnd A (ENot b)) c1 B ->
+    ht_ded A (If b c0 c1) B
+| ht_while : forall (A : EBExp) (b : BExp) (c : Cmd),
+    ht_ded (EAnd A b) c A ->
+    ht_ded A (While b c) (EAnd A (ENot b))
+| ht_cons : forall (A A' B B' : EBExp) (c : Cmd),
+    sat (eimpl A A') -> ht_ded A' c B' -> sat (eimpl B' B) ->
+    ht_ded A c B
+. 
+
+Lemma ht_asgn_derived: forall (X : nat) (a : AExp) (A : EBExp),
+    X ∉ aloc_vars a ∪ bloc_vars A ->
+    ht_ded A (Asgn X a) (EAnd A (EAEq (EVar X) a)).
+Proof.
+    intros * HX.
+    eapply ht_cons with (B' :=  (EAnd A (EAEq (EVar X) a)));
+        [| apply ht_asgn |]; cbn.
+    - rewrite fn_update_eq; cbn.
+      intros sigma I.
+      apply classical_satsi_impl.
+      intro HA.
+      rewrite satsi_and, satsi_eq.
+      rewrite bsubst_id, asubst_id; [done |..].
+      + rewrite subst_vars_fn_update_Some, subst_vars0.
+        apply equiv_empty; intros Y.
+        rewrite elem_of_intersection, elem_of_union, elem_of_singleton.
+        by intros [HYA [| ->]]; set_solver.
+      + by rewrite subst_vars0; set_solver.
+      + rewrite subst_vars_fn_update_Some, subst_vars0.
+        apply equiv_empty; intros Y.
+        rewrite elem_of_intersection, elem_of_union, elem_of_singleton.
+        by intros [HYA [| ->]]; set_solver.
+      + by rewrite subst_vars0; set_solver.
+    - by intros sigma I; apply classical_satsi_impl.
+Qed.
+
+Section sec_Hoare_logic_example.
+
+Context
+  (n s i : nat)
+  (Hns : n <> s)
+  (Hsi : s <> i)
+  (Hin : i <> n)
+  .
+
+Definition w : Cmd := 
+    While (ALe (Var i) (Var n))
+      (Seq
+      (Asgn s (Plus (Var s) (Var i)))
+      (Asgn i (Plus (Var i) (AVal 1)))).
+
+Definition p : Cmd :=
+  Seq (Seq
+  (Asgn s (AVal 0))
+  (Asgn i (AVal 0)))
+  w.
+
+Definition pre : BExp := ALe (AVal 0) (Var n).
+Definition post : BExp :=
+    AEq (Mul (AVal 2) (Var s)) (Mul (Var n) (Plus (Var n) (AVal 1))).
+
+Lemma step_1 : ht_ded
+    pre
+    (Asgn s (AVal 0))
+    (EAnd pre (EAEq (Var s) (AVal 0))).
+Proof. by apply ht_asgn_derived; set_solver. Qed.
+
+Lemma step_2 : ht_ded
+    (EAnd pre (EAEq (Var s) (AVal 0)))
+    (Asgn i (AVal 0))
+    (EAnd (EAnd pre (EAEq (Var s) (AVal 0))) (EAEq (Var i) (AVal 0))).
+Proof. by apply ht_asgn_derived; set_solver. Qed.
+
+Lemma step_12 : ht_ded
+    pre
+    (Seq (Asgn s (AVal 0)) (Asgn i (AVal 0)))
+    (EAnd (EAnd pre (EAEq (Var s) (AVal 0))) (EAEq (Var i) (AVal 0))).
+Proof.
+    eapply ht_seq; [apply step_1 | apply step_2].
+Qed.
+
+Definition invariant : BExp := And
+    (AEq (Mul (AVal 2) (Var s)) (Mul (Var i) (Minus (Var i) (AVal 1))))
+    (ALe (Var i) (Plus (Var n) (AVal 1))).
+
+Lemma loop_inv_1 : ht_ded
+    (bsubst invariant subst0 (mk_subst [(i, Plus (Var i) (AVal 1))]))
+    (Asgn i (Plus (Var i) (AVal 1)))
+    invariant.
+Proof. by apply ht_asgn. Qed.
+
+Lemma loop_inv_2 : ht_ded
+    (bsubst
+      (bsubst invariant subst0 (mk_subst [(i, Plus (Var i) (AVal 1))]))
+      subst0 (mk_subst [(s, Plus (Var s) (Var i))]))
+    (Asgn s (Plus (Var s) (Var i)))
+    (bsubst invariant subst0 (mk_subst [(i, Plus (Var i) (AVal 1))])).
+Proof. by apply ht_asgn. Qed.
+
+Lemma loop_inv_12 : ht_ded
+    (bsubst
+      (bsubst invariant subst0 (mk_subst [(i, Plus (Var i) (AVal 1))]))
+      subst0 (mk_subst [(s, Plus (Var s) (Var i))]))
+    (Seq
+      (Asgn s (Plus (Var s) (Var i)))
+      (Asgn i (Plus (Var i) (AVal 1))))
+    invariant.
+Proof.
+    eapply ht_seq; [apply loop_inv_2 | apply loop_inv_1].
+Qed.
+
+Lemma loop_inv : ht_ded
+    (EAnd invariant (ALe (Var i) (Var n)))
+    (Seq
+      (Asgn s (Plus (Var s) (Var i)))
+      (Asgn i (Plus (Var i) (AVal 1))))
+    invariant.
+Proof.
+    eapply ht_cons with (B' := invariant);
+      [| apply loop_inv_12 | by intros sigma I; apply classical_satsi_impl].
+    intros sigma I.
+    apply classical_satsi_impl.
+    unfold invariant; cbn.
+    rewrite !satsi_and, !satsi_eq, !satsi_le, !fn_update_eq.
+    unfold fn_update.
+    rewrite !decide_False by done; cbn.
+    rewrite decide_True by done.
+    rewrite !decide_False by done; cbn.
+    by nia.
+Qed.
+
+Lemma p_while : ht_ded
+    (EAnd (EAnd pre (EAEq (Var s) (AVal 0))) (EAEq (Var i) (AVal 0)))
+    w
+    post.
+Proof.
+    eapply ht_cons; [| apply ht_while, loop_inv |];
+      intros sigma I; apply classical_satsi_impl.
+    - unfold invariant; cbn; rewrite !satsi_and, !satsi_eq, !satsi_le; cbn.
+      by lia.
+    - unfold invariant; cbn; rewrite !satsi_and, satsi_not, !satsi_eq, !satsi_le; cbn.
+      by nia.
+Qed.
+
+Lemma p_correct : ht_ded pre p post.
+Proof.
+    by eapply ht_seq; [apply step_12 | apply p_while].
+Qed.
+
+End sec_Hoare_logic_example.
+    
